src/examples/transaction.v
@@ -134,212 +134,100 @@ Proof.
   eapply DR_RW; eauto.
 Qed.
 
-Lemma transaction_atomic_step:
-  forall p env tid s1 c1 ts1 mmts1 tr mach1 mach2 s2 c2 ts2 mmts2,
-    p = prog_intro env (IdMap.add tid transaction (IdMap.empty _)) ->
-    (forall tid', tid' =/= tid -> IdMap.find tid' mach1.(Machine.tmap) = None) ->
-    IdMap.find tid mach1.(Machine.tmap) = Some (Thread.mk s1 c1 ts1 mmts1) ->
-    suffix_of s1 transaction ->
-    consistent_state mach1.(Machine.mem) ->
-    Machine.step p tr mach1 mach2 ->
-    IdMap.find tid mach2.(Machine.tmap) = Some (Thread.mk s2 c2 ts2 mmts2) ->
-  suffix_of s2 transaction /\ consistent_state mach2.(Machine.mem).
-Proof.
-  i. subst. inv H4.
-  - split; ss.
-    destruct (tid0 == tid); cycle 1.
-    { apply H0 in c. rewrite c in THR1. ss. }
-    inv e. rewrite IdMap.add_spec in *. des_ifs.
-    inv THR_STEP; inv STEP; inv THR2; ss.
-    + inv H2. clear - H. unfold transaction in H.
-      rewrite app_comm_cons' in H. rewrite <- app_assoc in H.
-      destruct x; ss. inv H.
-      destruct x; ss. inv H2.
-      destruct x; ss. inv H1.
-      destruct x; ss. inv H2.
-      destruct x; ss.
-    + (* CAS-REPLAY *)
-      etrans; eauto. rewrite STMT. esplit. instantiate (1 := [_]). ss.
-    + inv H2. clear - H. unfold transaction in H.
-      rewrite app_comm_cons' in H. rewrite <- app_assoc in H.
-      destruct x; ss. inv H.
-      destruct x; ss. inv H2.
-      destruct x; ss. inv H1.
-      destruct x; ss. inv H2.
-      destruct x; ss.
-    + inv H2. clear - H. unfold transaction in H.
-      rewrite app_comm_cons' in H. rewrite <- app_assoc in H.
-      destruct x; ss. inv H.
-      destruct x; ss. inv H2.
-      destruct x; ss. inv H1.
-      destruct x; ss. inv H2.
-      destruct x; ss.
-    + inv H2. clear - H. unfold transaction in H.
-      rewrite app_comm_cons' in H. rewrite <- app_assoc in H.
-      destruct x; ss. inv H.
-      destruct x; ss. inv H2.
-      destruct x; ss. inv H1.
-      destruct x; ss. inv H2.
-      destruct x; ss.
-    + inv H2. clear - H. unfold transaction in H.
-      rewrite app_comm_cons' in H. rewrite <- app_assoc in H.
-      destruct x; ss. inv H.
-      destruct x; ss. inv H2.
-      destruct x; ss. inv H1.
-      destruct x; ss. inv H2.
-      destruct x; ss.
-    + inv H2. clear - H. unfold transaction in H.
-      rewrite app_comm_cons' in H. rewrite <- app_assoc in H.
-      destruct x; ss. inv H.
-      destruct x; ss. inv H2.
-      destruct x; ss. inv H1.
-      destruct x; ss. inv H2.
-      destruct x; ss.
-    + inv H2. clear - H. unfold transaction in H.
-      rewrite app_comm_cons' in H. rewrite <- app_assoc in H.
-      destruct x; ss. inv H.
-      destruct x; ss. inv H2.
-      destruct x; ss. inv H1.
-      destruct x; ss. inv H2.
-      destruct x; ss.
-    + inv H2. clear - H. unfold transaction in H.
-      rewrite app_comm_cons' in H. rewrite <- app_assoc in H.
-      destruct x; ss. inv H.
-      destruct x; ss. inv H2.
-      destruct x; ss. inv H1.
-      destruct x; ss. inv H2.
-      destruct x; ss.
-    + inv H2. clear - H. unfold transaction in H.
-      rewrite app_comm_cons' in H. rewrite <- app_assoc in H.
-      destruct x; ss. inv H.
-      destruct x; ss. inv H2.
-      destruct x; ss. inv H1.
-      destruct x; ss. inv H2.
-      destruct x; ss.
-    + inv H2. clear - H. unfold transaction in H.
-      rewrite app_comm_cons' in H. rewrite <- app_assoc in H.
-      destruct x; ss. inv H.
-      destruct x; ss. inv H2.
-      destruct x; ss. inv H1.
-      destruct x; ss. inv H2.
-      destruct x; ss.
-  - destruct (tid0 == tid); cycle 1.
-    { apply H0 in c. rewrite c in THR1. ss. }
-    inv e. ss. rewrite IdMap.gss in *. inv H5.
-    rewrite THR1 in H1. inv H1.
-    inv THR_STEP; inv STEP; inv MEM_STEP; inv EVENT; inv THR2; ss; subst.
-    + inv H2. clear - H. unfold transaction in H.
-      destruct x; ss. inv H.
-      destruct x; ss. inv H2.
-      destruct x; ss. inv H1.
-      destruct x; ss. inv H2.
-      destruct x; ss.
-    + inv H2. clear - H. unfold transaction in H.
-      destruct x; ss. inv H.
-      destruct x; ss. inv H2.
-      destruct x; ss. inv H1.
-      destruct x; ss. inv H2.
-      destruct x; ss.
-    + (* CAS-SUCC *)
-      split.
-      { etrans; eauto. esplit. instantiate (1 := [_]). ss. }
-      inv H2. unfold transaction in H. destruct x; ss.
-      { inv H. ss. }
-      inv H. destruct x; ss.
-      { inv H5. ii. rewrite fun_add_spec in H. des_ifs.
-        admit.
-        (* Contra: loc 1000 is non-zero by IH. *)
-      }
-      inv H5. destruct x; ss.
-      {
-        inv H2. ii. rewrite fun_add_spec in H. des_ifs.
-        admit.
-        (* Contra: loc 1000 is non-zero by IH. *)
-      }
-      inv H2. destruct x; ss.
-      { inv H5. ii. rewrite fun_add_spec in H. des_ifs; cycle 1.
-        { exfalso. apply c. ss. }
-        admit.
-        (* Contra: loc 1000 is non-zero by IH. *)
-      }
-      inv H5. destruct x; ss.
-    + (* CAS-FAIL *)
-      admit.
-  - split; [|ss].
-    ss. rewrite IdMap.add_spec in H5. des_ifs. inv e.
-    rewrite IdMap.gss in STMT. inv STMT. refl.
-Qed.
-
-Lemma thread_nexist:
-  forall p tid tr mach mach_term,
-    IdMap.find tid mach.(Machine.tmap) = None ->
-    Machine.rtc p tr mach mach_term ->
-  IdMap.find tid mach_term.(Machine.tmap) = None.
-Proof.
-  i. revert tid H. induction H0; i; ss. apply IHrtc.
-  inv ONE; ss.
-  - rewrite IdMap.add_spec. des_ifs.
-    inv e. rewrite H in THR1. ss.
-  - rewrite IdMap.add_spec. des_ifs.
-    inv e. rewrite H in THR1. ss.
-  - rewrite IdMap.add_spec. des_ifs.
-    inv e. rewrite H in THR1. ss.
-Qed.
-
-Lemma transaction_atomic_rtc_step:
-  forall p env tid s c ts mmts tr mach mach_term,
-    p = prog_intro env (IdMap.add tid transaction (IdMap.empty _)) ->
-    (forall tid', tid' =/= tid -> IdMap.find tid' mach.(Machine.tmap) = None) ->
-    IdMap.find tid mach.(Machine.tmap) = Some (Thread.mk s c ts mmts) ->
-    suffix_of s transaction ->
-    consistent_state mach.(Machine.mem) ->
-    Machine.rtc p tr mach mach_term ->
-  consistent_state mach_term.(Machine.mem).
-Proof.
-  i. revert env s c ts mmts H3 H2 H1 H0 H. induction H4; i; [ ss |]. subst.
-
-  hexploit Machine.step_preserves_thr; eauto. i. des.
-  remember thr2. dup H. rewrite Heqt in H. destruct t.
-
-  hexploit transaction_atomic_step; try exact ONE; eauto. i. des.
-  eapply IHrtc; eauto.
-  i.
-  eapply thread_nexist; eauto.
-  econs; eauto. econs.
-Qed.
-
-Theorem transaction_atomic:
+Theorem transaction_atomic_no_crash:
   forall p tid env tr mach_term,
     p = prog_intro env (IdMap.add tid transaction (IdMap.empty _)) ->
-    Machine.rtc p tr (Machine.init p) mach_term ->
+    Machine.rtc Machine.normal p tr (Machine.init p) mach_term ->
   consistent_state mach_term.(Machine.mem).
 Proof.
   i.
   assert (INIT_CONST: consistent_state (Machine.init p).(Machine.mem)).
   { left. ss. }
-  assert (SINGLE_THREAD: forall tid', tid' =/= tid -> IdMap.find tid' (Machine.init p).(Machine.tmap) = None).
-  { i. subst. unfold Machine.init.
-    rewrite IdMap.fold_1. ss. rewrite IdMap.add_empty. ss.
-    rewrite IdMap.add_spec. des_ifs.
-    apply IdMap.gempty.
+  inv H0; ss. inv ONE; ss.
+  { symmetry in PROG. inv PROG.
+    rewrite IdMap.fold_1 in *. rewrite IdMap.add_empty in *. ss.
+    rewrite IdMap.add_spec in *. des_ifs; cycle 1.
+    { rewrite IdMap.gempty in THR1. ss. }
+    inv THR_STEP; inv STEP; ss.
+    inv STMT. inv MMT. ss. lia.
   }
-  subst.
-  cut (
-    exists thr,
-      IdMap.find tid
-        (Machine.tmap (Machine.init (prog_intro env (IdMap.add tid transaction (IdMap.empty (list Stmt))))))
-      = Some thr
-      /\ transaction = thr.(Thread.stmt)).
-  { i. des. destruct thr.
-    eapply transaction_atomic_rtc_step; eauto.
-    ss. subst. refl.
+  symmetry in PROG. inv PROG.
+  rewrite IdMap.fold_1 in *. rewrite IdMap.add_empty in *. ss.
+  rewrite IdMap.add_spec in *. des_ifs; cycle 1.
+  { rewrite IdMap.gempty in THR1. ss. }
+  inv e. rewrite IdMap.add_add in *.
+  inv THR_STEP; inv STEP; inv STMT; inv MEM_STEP; ss; cycle 1.
+  { inv EVENT. ss. }
+  inv EVENT.
+
+  inv RTC; ss. inv ONE; ss.
+  { symmetry in PROG. inv PROG.
+    rewrite IdMap.add_spec in *. des_ifs; cycle 1.
+    { rewrite IdMap.gempty in THR1. ss. }
+    inv THR_STEP; inv STEP; ss.
+    inv STMT. inv MMT0. ss. lia.
+  }
+  symmetry in PROG. inv PROG.
+  rewrite IdMap.add_spec in *. des_ifs; cycle 1.
+  { rewrite IdMap.gempty in THR1. ss. }
+  inv e. rewrite IdMap.add_add in *.
+  inv THR_STEP; inv STEP; inv STMT; inv MEM_STEP; ss; cycle 1.
+  { inv EVENT. ss. }
+  inv EVENT.
+
+  inv RTC0; ss. inv ONE; ss.
+  { symmetry in PROG. inv PROG.
+    rewrite IdMap.add_spec in *. des_ifs; cycle 1.
+    { rewrite IdMap.gempty in THR1. ss. }
+    inv THR_STEP; inv STEP; ss.
+    inv STMT. inv MMT1. ss. lia.
+  }
+  symmetry in PROG. inv PROG.
+  rewrite IdMap.add_spec in *. des_ifs; cycle 1.
+  { rewrite IdMap.gempty in THR1. ss. }
+  inv e. rewrite IdMap.add_add in *.
+  inv THR_STEP; inv STEP; inv STMT; inv MEM_STEP; ss; cycle 1.
+  { inv EVENT. ss. }
+  inv EVENT.
+
+  inv RTC; ss. inv ONE; ss.
+  { symmetry in PROG. inv PROG.
+    rewrite IdMap.add_spec in *. des_ifs; cycle 1.
+    { rewrite IdMap.gempty in THR1. ss. }
+    inv THR_STEP; inv STEP; ss.
+    inv STMT. inv MMT2. ss. lia.
+  }
+  symmetry in PROG. inv PROG.
+  rewrite IdMap.add_spec in *. des_ifs; cycle 1.
+  { rewrite IdMap.gempty in THR1. ss. }
+  inv e. rewrite IdMap.add_add in *.
+  inv THR_STEP; inv STEP; inv STMT; inv MEM_STEP; ss; cycle 1.
+  { inv EVENT. ss. }
+  inv EVENT.
+
+  inv RTC0; ss; cycle 1.
+  { inv ONE; ss.
+    { symmetry in PROG. inv PROG.
+      rewrite IdMap.add_spec in *. des_ifs; cycle 1.
+      { rewrite IdMap.gempty in THR1. ss. }
+      inv THR_STEP; inv STEP; inv STMT; ss.
+    }
+    symmetry in PROG. inv PROG.
+    rewrite IdMap.add_spec in *. des_ifs; cycle 1.
+    { rewrite IdMap.gempty in THR1. ss. }
+    inv THR_STEP; inv STEP; inv STMT; ss.
   }
 
-  cut (IdMap.elements (IdMap.add tid transaction (IdMap.empty (list Stmt))) = [(tid, transaction)]).
-  { intro ELEM. ss.
-    rewrite IdMap.fold_1. rewrite ELEM. ss.
-    rewrite IdMap.gss. eauto.
-  }
+  ii. repeat rewrite fun_add_spec in *; des_ifs; eauto.
+  - exfalso. apply c2. ss.
+  - exfalso. apply c1. ss.
+Qed.
 
-  apply IdMap.add_empty.
+Theorem transaction_atomic:
+  forall p tid env tr mach_term,
+    p = prog_intro env (IdMap.add tid transaction (IdMap.empty _)) ->
+    Machine.rtc Machine.step p tr (Machine.init p) mach_term ->
+  consistent_state mach_term.(Machine.mem).
+Proof.
+  admit.
 Qed.
